theories/modules/SMod.v
@@ -24,10 +24,9 @@ Module SMod. Section SMOD.
   }.
 
   Definition wf (ms : t) : Prop :=
-    ∀ fno msk scp fspo bd
-       (FIND: alist_find fno (fnsems ms) = Some (msk, scp, (fspo, bd)))
-       (COND: fno = None),
-      fspo = None.
+    ∀ fno img msk scp fspo bd
+      (FIND: alist_find fno (fnsems ms) = Some (img, msk, scp, (fspo, bd))),
+      img = true ∧ is_some fspo ∧ (fno = None → fspo = Some (fspec_trivial)).
 
   (**** Linking ****)
   Program Definition empty : t := {|
@@ -109,8 +108,8 @@ Module SMod. Section SMOD.
     initial_st := ms.(initial_st);
   |}.
   Next Obligation.
-    i. destruct ms. ss. ii. unfold fnsems_scopes in *. unfold map_snd in*.
-    rewrite alist_find_map in H0. specialize (well_scoped_fns0 fn a).
+    i. destruct ms. ss. ii. unfold fnsems_scopes in *. unfold map_snd in *.
+    rewrite !alist_find_map in H0. specialize (well_scoped_fns0 fn a).
     destruct (alist_find fn fnsems0) eqn: E; try rewrite E in H0; ss.
     destruct f. destruct p. et.
   Qed.
@@ -180,9 +179,8 @@ Section Aux.
   (* Definition has_trivial_spec (md : SMod.t) (fn : string) : Prop := *)
   (*   ∃ fno msk scp, has_param md fno false msk scp ∧ msk fn. *)
 
-
-  (* Definition img_forall (md: SMod.t) : Prop := *)
-  (*   ∀ fno fnsem, alist_find fno (SMod.fnsems md) = Some fnsem -> fnsem.1.1.1. *)
+  (* Definition has_spec_forall (md: SMod.t) : Prop := *)
+  (*   ∀ fno fnsem, alist_find fno (SMod.fnsems md) = Some fnsem -> is_some fnsem.2.1. *)
 
   (* Definition spec_type_agree (md: SMod.t) (sp: sp_type) : Prop := *)
   (*   ∀ fn, is_spawn_ospec (sp fn) = is_spawn_ospec ((sp_from md) fn). *)
@@ -222,4 +220,4 @@ End Aux.
 (* Global Hint Unfold has_param : core. *)
 (* Global Hint Unfold has_trivial_spec : core. *)
 (* Global Hint Unfold spec_type_agree : core. *)
-(* Global Hint Unfold img_forall : core. *)
+(* Global Hint Unfold has_spec_forall : core. *)
