theories/cancellation/CancelMain.v
@@ -1,0 +1,82 @@
+Require Import CRIS.
+Require Import LMod LModTr GSim GSimFacts GSimTactics.
+Require Import MInline MInlineIntro MInlineElim ElimRel.
+(* Require Import CancelCore CancelPG CancelAG CancelSpawn CancelPre CancelPost. *)
+
+Set Implicit Arguments.
+
+Module MainSMod. Section MainSMod.
+
+  (*** Mod to lmod modification is required : not below... ***)
+
+  Context `{!crisG Γ Σ α β τ _S _I, !concG}.
+
+  Program Definition to_mod (sp : sp_type) (ms : SMod.t) : Mod.t := {|
+    Mod.scopes := ms.(SMod.scopes);
+    Mod.fnsems := List.map (λ '(fno, fnsem), (fno, SModTr.trans_ktree (if is_some fno then sp else sp_none) fnsem)) ms.(SMod.fnsems);
+    Mod.initial_st := ms.(SMod.initial_st);
+    |}.
+  Next Obligation.
+    i. destruct ms. ss. ii. unfold fnsems_scopes in *.
+    set (m:=map _) in H0.
+    replace (alist_find fn (m fnsems)) with (o_map (alist_find fn fnsems) (λ fnsem, SModTr.trans_ktree (if fn then sp else sp_none) fnsem)) in H0; cycle 1.
+    { subst m. destruct (alist_find fn fnsems) eqn:E; ss; des_ifs; rewrite -Heq; clear -E; induction fnsems; ss; des_ifs;
+          try (by destruct o; ss); try (by rewrite IHfnsems; eauto). }
+    specialize (well_scoped_fns fn a).
+    destruct (alist_find fn fnsems) eqn: E; ss.
+    destruct f. et.
+  Qed.
+  Next Obligation. ii. destruct ms. ss. eauto. Qed.
+  Next Obligation. ii. destruct ms. ss. eauto. Qed.
+
+End MainSMod. End MainSMod.
+
+Module CancelMain. Section CancelMain.
+
+Context `{_crisG: !crisG Γ Σ α β τ _S _I, _concG: !concG}.
+
+Lemma cancel_main md rs
+  (WFS: SMod.wf md)
+  (WF: Mod.wf (SMod.to_mod sp_none (SMod.cancel md)))
+  (VALID: ✓ rs)
+  :  
+  refines_lmod
+    (Mod.to_lmod (MInline.inline (MainSMod.to_mod (sp_from md) md)) rs)
+    (Mod.to_lmod (MInline.inline (SMod.to_mod (sp_from md) md)) rs).
+Proof using.
+  r. intro arg. eapply gsim_adequacy.
+  instantiate (1:= smj_top). instantiate (1:= smj_top).
+  unfold LMod.compile. s. rewrite /ITree.map /LModTr.trans /LModTr.interp_callE.  
+
+  rewrite !alist_find_map_snd.
+  set (fnsems := SMod.fnsems md).
+  set (m := map _).
+  replace (alist_find None (m fnsems)) with (o_map (alist_find None fnsems) (λ fnsem, SModTr.trans_ktree sp_none fnsem)); cycle 1.
+  { subst m. destruct (alist_find None fnsems) eqn: E; ss;
+      induction fnsems; ss; des_ifs; try (destruct o; ss); try (rewrite IHfnsems; ss). }
+  subst m fnsems.
+  destruct (alist_find None (SMod.fnsems md)) eqn: FIND; cycle 1.
+  { s. ired. ginit. gstep. econs. econs. ss. }
+  s. ired. rewrite /ModTr.trans_ktree.
+  destruct f as [[[img msk] scp] [fspo bd]]. s.
+  assert (SCP: incl scp (SMod.scopes md)).
+  { ii. eapply SMod.well_scoped_fns. rewrite /fnsems_scopes. erewrite FIND. et. }
+  erewrite !sandbox_inline_commute; et.
+  rewrite /SB.sandbox_body. s.
+
+  ginit. guclo bindC_spec. econs; cycle 1.
+  { instantiate (1:=cancel_eq). i. gstep. econs. econs.
+    destruct SIM. des. et. }
+
+  r in WFS. hexploit WFS; eauto; i; des; ss.
+  hexploit H1; eauto; i; subst; ss.
+
+  ziter_l. zstep_l. ziter_l. zstep_l.
+  exploit WFS; et. i; des; subst; ss.
+  
+  
+  ginit. guclo bindC_spec. econs; cycle 1.
+  { instantiate (1:=cancel_eq). i. gstep. econs. econs.
+    destruct SIM. des. et. }
+  ziter_l. zstep_l. ziter_l. zstep_l.
+  exploit WFS; et. i; des; subst; ss.
