theories/cancellation/CancelSpawn.v
@@ -5,182 +5,91 @@ Require Import MInline MInlineIntro MInlineElim ElimRel.
 Lemma cancel_spawn `{_crisG: !crisG Γ Σ α β τ _S _I, _concG: !concG} md sp fn args :
   CANCEL_GOAL md sp (NativeSpawnE fn args) (HoareSpawnE fn args (sp fn)).
 Proof.
-  r; i. assert (VP0:=VP). destruct VP0 as [VP1 VP2]. r in VP1.
-  rewrite /sp_from /to_sp in VP1. setoid_rewrite alist_find_map_snd in VP1.
+  r; i. subst.
+  (* rewrite /sp_from /to_sp in WFS. setoid_rewrite alist_find_map_snd in WFS. *)
   ziter_l. ziter_r. rewrite x0 x1 /=. zstep_l.
   rewrite !alist_find_map_snd.
   destruct (alist_find (Some fn) (SMod.fnsems md)) eqn: FIND; rewrite !FIND; cycle 1.
   { s. zstep_l. }
-  destruct f as [[msk scp] [fspo bd]].
+  destruct f as [[[img msk] scp] [fspo bd]].
   assert (WFSCP: incl scp (SMod.scopes md)).
   { etrans; [|apply SMod.well_scoped_fns].
     rewrite /fnsems_scopes. erewrite FIND. refl.
   }
 
-  destruct (sp fn) eqn: E; s; cycle 1.
-  { des. specialize (VP2 fn). rewrite E /sp_from /to_sp alist_find_map_snd FIND /= in VP2.
-    destruct fspo; ss. destruct f; ss. r in VP0. hexploit VP0; eauto. i; ss. }
-  { (* the spawnee has a non-trivial spec *)
-    destruct f.
-    { ired. zstep_r. }
-    destruct fspo; cycle 1.
-    { des. r in VP0. hexploit VP0; eauto; i; ss. }
-    destruct f.
-    { des. specialize (VP2 fn). rewrite E /sp_from /to_sp alist_find_map_snd FIND // in VP2. }
-    ired. ziter_l. zstep_l.
-    do 2 zstep_r.
-    ziter_r; zstep_r.
-    ziter_r; do 2 zstep_r.
-    ziter_r; zstep_r.
-    ziter_r; zstep_r.
-    rewrite !alist_find_map_snd FIND /=. ired.
-    ziter_r; zstep_r.
-    ziter_r; zstep_r.
-    ziter_r; zstep_r.
-    rewrite YieldToken_gen in RS.
-    hexploit (Own_bupd_split).
-    { iIntros "S". iPoseProof (RS with "S") as ">(D & R & TA & T & [YA NY] & Y & W)".
-      iModIntro. iCombine "D TA T YA Y W" as "P". iCombine "R NY" as "Q".
-      iSplitL "P"; [iApply "P"|iApply "Q"]. }
-    { eauto. }
-    intros [r_t1 [r_t2 [Hr_t [Hr_t1 Hr_t2]]]].
-    exists r_t2. zstep_r.
-    ziter_r; zstep_r.
-    assert (RES: ✓ r_t2 ∧ (Own r_t2 ⊢ |==> YIELD (length tgts) ∗ Own r_t)).
-    { split; eauto.
-      { eapply Own_wand_valid; [iIntros "S"; iMod (Hr_t with "S") as "[_ $]"; done|eauto]. }
-      { rewrite Hr_t2 EQLEN2 EQLEN. iIntros "[$ $]"; done. }
-    }
-    exists RES.
-    zstep_r.
-    do 4 (ziter_r; zstep_r).
-    ziter_r; do 2 zstep_r.
-    ziter_r; do 2 zstep_r.
-    do 3 (ziter_r; zstep_r).
-    zprogress. gbase.
-    des; hexploit (Own_bupd_split); et.
-    intros [r_t3 [r_t4 [Hr_t3 [Hr_t4 Hr_t5]]]].
-    eapply CIH; eauto.
-    { rewrite -!insert_app_l; try lia.
-      instantiate (1:=<[cid:=ε]>(rs_diff ++ [r_t3])).
-      econs; first (rewrite !length_insert !length_app /=; lia).
-      econs; first (rewrite !length_insert !length_app /=; lia).
-      intros i ???; destruct (decide (i = cid)).
-      { subst; rewrite ?list_lookup_insert; try (rewrite length_app /=; lia).
-        do 3 (intros INV; inv INV).
-        econs; eauto. rewrite -EQLEN; eapply KTR.
-      }
-      rewrite !list_lookup_insert_ne //.
-      destruct (decide (i < length srcs)).
-      { rewrite !lookup_app_l; try lia. ii; eapply REL; eauto. }
-      destruct (decide (i = length srcs)); cycle 1.
-      { rewrite ?lookup_ge_None_2; ss; rewrite ?length_app /=; lia. }
-      subst; rewrite list_lookup_length EQLEN list_lookup_length -EQLEN -EQLEN2 list_lookup_length.
-      do 3 (intros INV; inv INV).
-
-      rewrite /ModTr.trans_ktree !sandbox_inline_commute /SB.sandbox_body; try by eauto.
-      rewrite /SModTr.trans_ktree /SModTr.trans_body.
-      replace (SModTr.HoareFun (Some _)) with (Seal.sealing "temp" (SModTr.HoareFun (Some (fspec_spawn precond0 postcond0)))); cycle 1.
-      { unseal "temp". refl. }
-      ss. unseal "temp".
-      rewrite (@MIRed_HoareFun _ _ _ _ _ _ _ _ _ md sp msk scp bd (Some (fspec_spawn precond0 postcond0)) x3 fn meta0 precond0 postcond0); eauto.
-      rewrite SBRed.tau MIRed.tau.
-      hexploit (VP1 fn); rewrite FIND /=; revert E; intros ->; ss; intros Himp.
-      hexploit (Himp (length tgts) x); intros [x' [PRE ?]].
-      eapply thread_rel_spawn; eauto.
-      { destruct rs_diff; ss. }
-      { iIntros "X //". iPoseProof (Hr_t4 with "X") as "X".
-        rewrite EQLEN2 EQLEN. unfold FSpec.precond, FSpec.postcond in *.
-        iMod (PRE with "X") as "X"; done.
-      }
-      { ss; eapply elim_rel_cancel; eauto. }
-    }
-    rewrite insert_app_l; last lia.
-    rewrite Hr_t Hr_t1 Hr_t3 Hr_t5 list_insert_id // big_sepL_app /= right_id last_length.
-    iIntros ">(($ & $) & >[$ $])"; done.
+  assert (EQ: sp_from md fn = fspo).
+  { rewrite /sp_from /to_sp alist_find_map_snd /= FIND //. }
+  rewrite !EQ /=.
+  r in WFS. hexploit WFS; eauto; i; ss; des; subst img.
+  destruct fspo; ss. destruct f.
+  { ired. zstep_r. }
+    
+  ired. ziter_l. zstep_l.
+  do 2 zstep_r.
+  ziter_r; zstep_r.
+  ziter_r; do 2 zstep_r.
+  ziter_r; zstep_r.
+  ziter_r; zstep_r.
+  rewrite !alist_find_map_snd FIND /=. ired.
+  ziter_r; zstep_r.
+  ziter_r; zstep_r.
+  ziter_r; zstep_r.
+  rewrite YieldToken_gen in RS.
+  hexploit (Own_bupd_split).
+  { iIntros "S". iPoseProof (RS with "S") as ">(D & R & TA & T & [YA NY] & Y & W)".
+    iModIntro. iCombine "D TA T YA Y W" as "P". iCombine "R NY" as "Q".
+    iSplitL "P"; [iApply "P"|iApply "Q"]. }
+  { eauto. }
+  intros [r_t1 [r_t2 [Hr_t [Hr_t1 Hr_t2]]]].
+  exists r_t2. zstep_r.
+  ziter_r; zstep_r.
+  assert (RES: ✓ r_t2 ∧ (Own r_t2 ⊢ |==> YIELD (length tgts) ∗ Own r_t)).
+  { split; eauto.
+    { eapply Own_wand_valid; [iIntros "S"; iMod (Hr_t with "S") as "[_ $]"; done|eauto]. }
+    { rewrite Hr_t2 EQLEN2 EQLEN. iIntros "[$ $]"; done. }
   }
-      (* Experimental *)
-      (* rewrite interpV_bind.
-      set (ktr := λ x8, interpV _ _).
-      eapply (eq_ind ktr); cycle 1.
-      { subst ktr; extensionalities x8; destruct x8.
-        rewrite interpV_bind.
-        (* Set Printing All. *)
-        instantiate (1:= λ x,
-          vret <- interpV ModTr.handle_hmodE (inline_body (sandboxed_prog (SMod.to_hmod sp md)) (SB.sandbox img msk scp (SModTr.trans (if img then sp else sp_none) (bd x.2))));;
-          interpV ModTr.handle_hmodE (elim_spawnee_postcond (fspo_post fspo) x.1 vret)).
-        ss.
-      }
-        subst ktr.
-      }
-      eapply eq_ind; cycle 1.
-        2:{ }
-      } *)
-      (* econs; eauto; cycle 1.
-      { rewrite (bind_ret_r_rev (interpV _ _)) //. }
-      hexploit (VP1 fn); rewrite FIND /=; revert E; destruct img0; ss; intros ->; ss; intros Himp.
-      hexploit (Himp x); intros [x' [PRE ?]].
-      pfold; eapply (elim_rel_spawnee_pre sp _ x'); last refl; ss; cycle 1.
-      { destruct fspo; ss; iIntros "X //". iApply PRE; iApply Hr_t1; done. }
-      left. ginit.
-      guclo elim_rel_bindC_spec; rewrite (bind_ret_r_rev (inline_body _ _)); econs; eauto.
-      { gfinal; right. eapply elim_rel_cancel; eauto. r; esplits; eauto. }
-      intros ?; gfinal; right; pfold; rewrite (bind_ret_r_rev (elim_spawnee_postcond _ _ _)).
-      eapply elim_rel_spawnee_post; eauto.
+  exists RES.
+  zstep_r.
+  do 4 (ziter_r; zstep_r).
+  ziter_r; do 2 zstep_r.
+  ziter_r; do 2 zstep_r.
+  do 3 (ziter_r; zstep_r).
+  zprogress. gbase.
+  des; hexploit (Own_bupd_split); et.
+  intros [r_t3 [r_t4 [Hr_t3 [Hr_t4 Hr_t5]]]].
+  eapply CIH; eauto.
+  { rewrite -!insert_app_l; try lia.
+    instantiate (1:=<[cid:=ε]>(rs_diff ++ [r_t3])).
+    econs; first (rewrite !length_insert !length_app /=; lia).
+    econs; first (rewrite !length_insert !length_app /=; lia).
+    intros i ???; destruct (decide (i = cid)).
+    { subst; rewrite ?list_lookup_insert; try (rewrite length_app /=; lia).
+      do 3 (intros INV; inv INV).
+      econs; eauto. rewrite -EQLEN; eapply KTR.
     }
-    rewrite insert_app_l; last lia.
-    rewrite list_insert_id // big_sepL_app /= right_id RS Hr_t Hr_t2.
-    iIntros "> [$ > [$ $]]"; done.
-  } *)
-  (* { (* fn has a trivial spec in sp *) *)
-  (*   ired. zstep_r. *)
-  (*   ziter_l; zstep_l. *)
-  (*   rewrite !alist_find_map_snd FIND /=; ired. *)
-  (*   ziter_r; zstep_r. *)
-  (*   zprogress. gbase. *)
-  (*   eapply CIH. *)
-  (*   { rewrite -!insert_app_l; try lia. *)
-  (*     instantiate (1:=<[cid:=ε]>(rs_diff ++ [ε])). *)
-  (*     econs; first (rewrite !length_insert !length_app /=; lia). *)
-  (*     econs; first (rewrite !length_insert !length_app /=; lia). *)
-  (*     intros i ???; destruct (decide (i = cid)). *)
-  (*     { subst; rewrite ?list_lookup_insert; try (rewrite length_app /=; lia). *)
-  (*       do 3 (intros INV; inv INV). *)
-  (*       econs; eauto. rewrite -EQLEN; eapply KTR. *)
-  (*     } *)
-  (*     rewrite !list_lookup_insert_ne //. *)
-  (*     destruct (decide (i < length srcs)). *)
-  (*     { rewrite !lookup_app_l; try lia. ii; eapply REL; eauto. } *)
-  (*     destruct (decide (i = length srcs)); cycle 1. *)
-  (*     { rewrite ?lookup_ge_None_2; ss; rewrite ?length_app /=; lia. } *)
-  (*     subst; rewrite list_lookup_length EQLEN list_lookup_length -EQLEN -EQLEN2 list_lookup_length. *)
-  (*     do 3 (intros INV; inv INV). *)
-  (*     rewrite /ModTr.trans_ktree !sandbox_inline_commute /SB.sandbox_body //=. *)
-  (*     rewrite (MIRed_HoareFun _ _ fn) //= if_simpl SBRed.tau MIRed.tau. *)
-  (*     (* econs; eauto; cycle 1. *)
-  (*     { rewrite bind_ret_r //. } *) *)
-  (*     (* rewrite !sandbox_inline_commute //. *)
-  (*     rewrite !if_simpl /SB.sandbox_body /= (MIRed_HoareFun _ _ fn) //. *) *)
+    rewrite !list_lookup_insert_ne //.
+    destruct (decide (i < length srcs)).
+    { rewrite !lookup_app_l; try lia. ii; eapply REL; eauto. }
+    destruct (decide (i = length srcs)); cycle 1.
+    { rewrite ?lookup_ge_None_2; ss; rewrite ?length_app /=; lia. }
+    subst; rewrite list_lookup_length EQLEN list_lookup_length -EQLEN -EQLEN2 list_lookup_length.
+    do 3 (intros INV; inv INV).
 
-  (*     assert (Himpl : fspec_imply (fspec_flat fspo) fspec_trivial). *)
-  (*     { hexploit (VP1 fn); rewrite FIND /=; intros Himpl. *)
-  (*       destruct img0. *)
-  (*       { rewrite E in Himpl; ss. } *)
-  (*       { etrans; eauto. } *)
-  (*     } *)
-  (*     hexploit (Himpl ()); intros [? [PRE ?]]. *)
-  (*     eapply thread_rel_spawn; eauto. *)
-  (*     { destruct rs_diff; ss. } *)
-  (*     { destruct fspo; ss. *)
-  (*       { iIntros "X //". iApply PRE; done. } *)
-  (*       { iIntros "X //". } *)
-  (*     } *)
-  (*     { ss; eapply elim_rel_cancel; eauto. } *)
-  (*   } *)
-  (*   { eauto. } *)
-  (*   { rewrite insert_app_l; last lia. *)
-  (*     rewrite list_insert_id // big_sepL_app /= right_id RS. *)
-  (*     iIntros "> [$ $] !>"; iApply Own_unit. *)
-  (*   } *)
-  (* } *)
+    rewrite /ModTr.trans_ktree !sandbox_inline_commute /SB.sandbox_body; try by eauto.
+    rewrite /SModTr.trans_ktree /SModTr.trans_body.
+    replace (SModTr.HoareFun) with (Seal.sealing "temp" (SModTr.HoareFun)); cycle 1.
+    { unseal "temp". refl. }
+    ss. unseal "temp".
+    rewrite (@MIRed_HoareFun _ _ _ _ _ _ _ _ _ md (sp_from md) true msk scp bd (Some (fspec_spawn precond postcond)) x3 (Some fn) meta precond postcond); eauto.
+    rewrite SBRed.tau MIRed.tau.
+    (* hexploit (VP1 fn); rewrite FIND /=; revert E; intros ->; ss; intros Himp. *)
+    (* hexploit (Himp (length tgts) x); intros [x' [PRE ?]]. *)
+    eapply thread_rel_spawn; eauto.
+    { destruct rs_diff; ss. }
+    { rewrite EQLEN2 EQLEN. iIntros "X //". iPoseProof (Hr_t4 with "X") as "X"; done. }
+    { ss; eapply elim_rel_cancel; eauto. }
+  }
+  rewrite insert_app_l; last lia.
+  rewrite Hr_t Hr_t1 Hr_t3 Hr_t5 list_insert_id // big_sepL_app /= right_id last_length.
+  iIntros ">(($ & $) & >[$ $])"; done.
 (*SLOW*)Qed.
